Phi_Semantics/PhiSem_CF_Breakable.thy
@@ -3,19 +3,22 @@ theory PhiSem_CF_Breakable
 begin
 
 
-
+text \<open>Since we have \<^verbatim>\<open>break\<close> and \<^verbatim>\<open>continue\<close> now, the termination condition of a loop is not
+  necessarily the negative of the loop guard. Therefore here we need 3 assertions, invariance,
+  guard, and termination condition.\<close>
 
 proc while:
-  assumes \<open>\<^bold>p\<^bold>a\<^bold>r\<^bold>a\<^bold>m (X x \<^bold>s\<^bold>u\<^bold>b\<^bold>j x. Inv: invariant x \<and> Guard: cond x)\<close>
+  assumes \<open>\<^bold>p\<^bold>a\<^bold>r\<^bold>a\<^bold>m (X x \<^bold>s\<^bold>u\<^bold>b\<^bold>j x. Inv: invariant x \<and> Guard: cond x \<and> End: termination x)\<close>
   and S: \<open>\<^bold>v\<^bold>i\<^bold>e\<^bold>w U \<longmapsto> (X x \<^bold>s\<^bold>u\<^bold>b\<^bold>j x. invariant x) @action ToSA\<close>
+  and \<open>\<^bold>p\<^bold>r\<^bold>e\<^bold>m\<^bold>i\<^bold>s\<^bold>e (\<forall>x. \<not> cond x \<longrightarrow> termination x)\<close>
   and C: "\<And>x. \<^bold>p\<^bold>r\<^bold>e\<^bold>m\<^bold>i\<^bold>s\<^bold>e invariant x \<Longrightarrow>
                   \<^bold>p\<^bold>r\<^bold>o\<^bold>c Cond \<lbrace> X x \<longmapsto> X x'\<heavy_comma> \<^bold>v\<^bold>a\<^bold>l cond x' \<Ztypecolon> \<bool> \<^bold>s\<^bold>u\<^bold>b\<^bold>j x'. invariant x' \<rbrace> \<^bold>t\<^bold>h\<^bold>r\<^bold>o\<^bold>w\<^bold>s E1"
   and B: "\<And>x lb lc. \<^bold>p\<^bold>r\<^bold>e\<^bold>m\<^bold>i\<^bold>s\<^bold>e invariant x \<Longrightarrow>
                     \<^bold>p\<^bold>r\<^bold>e\<^bold>m\<^bold>i\<^bold>s\<^bold>e cond x \<Longrightarrow>
                     break_\<phi>app\<^bold>: HIDDEN_PREM(
                         \<^bold>p\<^bold>r\<^bold>o\<^bold>c (op_break lb \<phi>V_none :: unit proc)
-                           \<lbrace> (X x'\<heavy_comma> Brk_Frame lc \<^bold>s\<^bold>u\<^bold>b\<^bold>j x'. invariant x' \<and> \<not> cond x')\<heavy_comma> Brk_Frame lb \<longmapsto> 0 \<rbrace>
-                        \<^bold>t\<^bold>h\<^bold>r\<^bold>o\<^bold>w\<^bold>s (\<lambda>_. Brking_Frame lb (\<lambda>_::unit \<phi>arg. X x'\<heavy_comma> Brk_Frame lc \<^bold>s\<^bold>u\<^bold>b\<^bold>j x'. invariant x' \<and> \<not> cond x'))) \<Longrightarrow>
+                           \<lbrace> (X x'\<heavy_comma> Brk_Frame lc \<^bold>s\<^bold>u\<^bold>b\<^bold>j x'. invariant x' \<and> termination x')\<heavy_comma> Brk_Frame lb \<longmapsto> 0 \<rbrace>
+                        \<^bold>t\<^bold>h\<^bold>r\<^bold>o\<^bold>w\<^bold>s (\<lambda>_. Brking_Frame lb (\<lambda>_::unit \<phi>arg. X x'\<heavy_comma> Brk_Frame lc \<^bold>s\<^bold>u\<^bold>b\<^bold>j x'. invariant x' \<and> termination x'))) \<Longrightarrow>
                     continue_\<phi>app\<^bold>: HIDDEN_PREM(
                         \<^bold>p\<^bold>r\<^bold>o\<^bold>c (op_break lc \<phi>V_none :: unit proc)
                            \<lbrace> (X x'\<heavy_comma> Brk_Frame lb \<^bold>s\<^bold>u\<^bold>b\<^bold>j x'. invariant x')\<heavy_comma> Brk_Frame lc \<longmapsto> 0 \<rbrace>
@@ -23,11 +26,11 @@ proc while:
                     \<^bold>p\<^bold>r\<^bold>o\<^bold>c Body lb lc
                         \<lbrace> X x\<heavy_comma> Brk_Frame lc\<heavy_comma> Brk_Frame lb
                       \<longmapsto> X x'\<heavy_comma> Brk_Frame lc\<heavy_comma> Brk_Frame lb \<^bold>s\<^bold>u\<^bold>b\<^bold>j x'. invariant x'
-                         \<rbrace> \<^bold>t\<^bold>h\<^bold>r\<^bold>o\<^bold>w\<^bold>s (\<lambda>e. \<^bold>b\<^bold>r\<^bold>e\<^bold>a\<^bold>k lb \<^bold>w\<^bold>i\<^bold>t\<^bold>h (\<lambda>_::unit \<phi>arg. X x'\<heavy_comma> Brk_Frame lc \<^bold>s\<^bold>u\<^bold>b\<^bold>j x'. invariant x' \<and> \<not> cond x')
+                         \<rbrace> \<^bold>t\<^bold>h\<^bold>r\<^bold>o\<^bold>w\<^bold>s (\<lambda>e. \<^bold>b\<^bold>r\<^bold>e\<^bold>a\<^bold>k lb \<^bold>w\<^bold>i\<^bold>t\<^bold>h (\<lambda>_::unit \<phi>arg. X x'\<heavy_comma> Brk_Frame lc \<^bold>s\<^bold>u\<^bold>b\<^bold>j x'. invariant x' \<and> termination x')
                                     \<^bold>o\<^bold>r \<^bold>b\<^bold>r\<^bold>e\<^bold>a\<^bold>k lc \<^bold>w\<^bold>i\<^bold>t\<^bold>h (\<lambda>_::unit \<phi>arg. X x' \<^bold>s\<^bold>u\<^bold>b\<^bold>j x'. invariant x')
                                     \<^bold>o\<^bold>r E2 e)"
   input \<open>U\<close>
-  output \<open>X x \<^bold>s\<^bold>u\<^bold>b\<^bold>j x. invariant x \<and> \<not> cond x\<close>
+  output \<open>X x \<^bold>s\<^bold>u\<^bold>b\<^bold>j x. invariant x \<and> termination x\<close>
   throws \<open>E1 + E2\<close>
   \<medium_left_bracket> S
     brk_scope \<medium_left_bracket> for lb
@@ -39,7 +42,7 @@ proc while:
           "_op_break_rule_"[THEN HIDDEN_PREM_I, THEN Labelled_I]
         \<medium_right_bracket> for \<open>(X x'\<heavy_comma> Brk_Frame lb \<^bold>s\<^bold>u\<^bold>b\<^bold>j x'. invariant x')\<heavy_comma> Brk_Frame lc\<close> .. ;;
       \<medium_right_bracket>. ;;
-    \<medium_right_bracket> for \<open>(X x' \<^bold>s\<^bold>u\<^bold>b\<^bold>j x'. invariant x' \<and> \<not> cond x')\<heavy_comma> Brk_Frame lb\<close> .. ;;
+      \<medium_right_bracket> for \<open>(X x' \<^bold>s\<^bold>u\<^bold>b\<^bold>j x'. invariant x' \<and> termination x')\<heavy_comma> Brk_Frame lb\<close> .. ;;
   \<medium_right_bracket>. .
 
 hide_const (open) PhiSem_CF_Basic.while
