Phi_Semantics/PhiSem_Play_Ground.thy
@@ -5,8 +5,6 @@ theory PhiSem_Play_Ground
     PhiSem_Variable
 begin
 
-thm while_\<phi>app
-
 (*
 proc
   assumes [\<phi>reason]: \<open>\<phi>SemType (x \<Ztypecolon> T) TY\<close>
@@ -37,18 +35,18 @@ setup \<open>Context.theory_map (Generic_Variable_Access.Process_of_Argument.put
 
 (* declare [[\<phi>hide_techinicals=false]] *)
 
+declare [[\<phi>hide_brk_frame]]
+
 proc
   input \<open>\<^bold>v\<^bold>a\<^bold>l x \<Ztypecolon> \<nat>[32]\<close>
   premises \<open>x < 10\<close>
   output \<open>\<^bold>v\<^bold>a\<^bold>l 10 \<Ztypecolon> \<nat>[32]\<close>
   \<medium_left_bracket>
     $x \<rightarrow> var v (*x is an immutable value, and here we assign it to a variable v*)
-    while \<open>x \<Ztypecolon> ?T \<^bold>s\<^bold>u\<^bold>b\<^bold>j x. Inv: (x \<le> 10) \<and> Guard: x < 10\<close> (*annotation*)
-    \<medium_left_bracket> \<open>$v < 10\<close> \<medium_right_bracket>. (*guard*)
-    \<medium_left_bracket> \<open>$v + 1\<close> \<rightarrow> v ;;
-      thm break_\<phi>app ;;
-      thm continue_\<phi>app ;;
-      if \<open>$v = 10\<close> \<medium_left_bracket> break \<medium_right_bracket>. \<medium_left_bracket> continue \<medium_right_bracket>. ;;
+    while \<open>x \<Ztypecolon> ?T \<^bold>s\<^bold>u\<^bold>b\<^bold>j x. Inv: (x \<le> 10) \<and> Guard: True \<and> End: (x = 10)\<close> (*annotation*)
+    \<medium_left_bracket> \<open>True\<close> \<medium_right_bracket>. (*guard*)
+    \<medium_left_bracket>
+      if \<open>$v = 10\<close> \<medium_left_bracket> break \<medium_right_bracket>. \<medium_left_bracket> \<open>$v + 1\<close> \<rightarrow> v;; continue \<medium_right_bracket>.
       assert \<bottom>
     \<medium_right_bracket>. (*loop body*)
     $v
